Examples/alpha_def.v
@@ -1,0 +1,34 @@
+From PlutusCert Require Import 
+  STLC
+  Alpha.alpha.
+Require Import Coq.Lists.List.
+Import ListNotations.
+
+Lemma alpha_exampl x y y' A :
+  x <> y -> y <> y' -> x <> y' -> 
+  Alpha [] (@tmabs Lam x A (@tmabs Lam y A (@tmbin App (tmvar x) (tmvar y)))) (@tmabs Lam y A (@tmabs Lam y' A (@tmbin App (tmvar y) (tmvar y')))).
+Proof.
+  intros Hxy Hyy' Hxy'.
+  apply alpha_lam.
+  apply alpha_lam.
+  apply alpha_app.
+  - apply alpha_var. apply alpha_var_diff; try symmetry; try assumption.
+    apply alpha_var_cons; reflexivity.
+  - apply alpha_var. apply alpha_var_cons; reflexivity.
+Qed.
+
+(* Showcasing shadowing behaviour is right *)
+Lemma alpha_counterexample x y z A :
+  x <> y -> x <> z -> y <> z -> 
+  (Alpha [] (@tmabs Lam x A (@tmabs Lam y A (@tmbin App (tmvar x) (tmvar y)))) 
+    (@tmabs Lam z A (@tmabs Lam z A (@tmbin App (tmvar z) (tmvar z)))) -> False).
+Proof.
+  intros Hxy Hxz Hyz Halpha.
+  inversion Halpha; subst.
+  inversion H1; subst.
+  inversion H2; subst.
+  inversion H4; subst.
+  inversion H5; subst.
+  - contradiction Hxy. subst. reflexivity. 
+  - contradiction.
+Qed.
